isabelle-thys/Programs.thy
@@ -17,25 +17,65 @@ consts
   measurement :: "'a variables \<Rightarrow> 'b variables \<Rightarrow> ('a,'b) measurement expression \<Rightarrow> program"
   instantiateOracles :: "oracle_program \<Rightarrow> program list \<Rightarrow> program"
 
-consts fv_oracle_program :: "oracle_program \<Rightarrow> string set"
+consts fvq_oracle_program :: "oracle_program \<Rightarrow> string set"
+consts fvc_oracle_program :: "oracle_program \<Rightarrow> string set"
+consts fvcw_oracle_program :: "oracle_program \<Rightarrow> string set"
 
-consts fv_program :: "program \<Rightarrow> string set"
-lemma fv_program_sequence: "fv_program (block b) = (\<Union>s\<in>set b. fv_program s)"
+consts fvq_program :: "program \<Rightarrow> string set"
+lemma fvq_program_sequence: "fvq_program (block b) = (\<Union>s\<in>set b. fvq_program s)"
   by (cheat TODO7)
-lemma fv_program_assign: "fv_program (assign x e) = set (variable_names x) \<union> fv_expression e"
+lemma fvq_program_assign: "fvq_program (assign x e) = {}"
   by (cheat TODO7)
-lemma fv_program_sample: "fv_program (sample xs e2) = set (variable_names xs) \<union> fv_expression e2"
+lemma fvq_program_sample: "fvq_program (sample xs e2) = {}"
   by (cheat TODO7)
-lemma fv_program_ifthenelse: "fv_program (ifthenelse c p1 p2) =
-  fv_expression c \<union> (\<Union>s\<in>set p1. fv_program s) \<union> (\<Union>s\<in>set p2. fv_program s)"
+lemma fvq_program_ifthenelse: "fvq_program (ifthenelse c p1 p2) =
+  (\<Union>s\<in>set p1. fvq_program s) \<union> (\<Union>s\<in>set p2. fvq_program s)"
   by (cheat TODO7)
-lemma fv_program_while: "fv_program (while c b) = fv_expression c \<union> (\<Union>s\<in>set b. fv_program s)"
+lemma fvq_program_while: "fvq_program (while c b) = (\<Union>s\<in>set b. fvq_program s)"
   by (cheat TODO7)
-lemma fv_program_qinit: "fv_program (qinit Q e3) = set (variable_names Q) \<union> fv_expression e3"
+lemma fvq_program_qinit: "fvq_program (qinit Q e3) = set (variable_names Q)"
   by (cheat TODO7)
-lemma fv_program_qapply: "fv_program (qapply Q e4) = set (variable_names Q) \<union> fv_expression e4"
+lemma fvq_program_qapply: "fvq_program (qapply Q e4) = set (variable_names Q)"
   by (cheat TODO7)
-lemma fv_program_measurement: "fv_program (measurement x R e5) = set (variable_names x) \<union> set (variable_names R) \<union> fv_expression e5"
+lemma fvq_program_measurement: "fvq_program (measurement x R e5) = set (variable_names R)"
+  by (cheat TODO7)
+
+consts fvc_program :: "program \<Rightarrow> string set"
+lemma fvc_program_sequence: "fvc_program (block b) = (\<Union>s\<in>set b. fvc_program s)"
+  by (cheat TODO7)
+lemma fvc_program_assign: "fvc_program (assign x e) = set (variable_names x) \<union> fv_expression e"
+  by (cheat TODO7)
+lemma fvc_program_sample: "fvc_program (sample xs e2) = set (variable_names xs) \<union> fv_expression e2"
+  by (cheat TODO7)
+lemma fvc_program_ifthenelse: "fvc_program (ifthenelse c p1 p2) =
+  fv_expression c \<union> (\<Union>s\<in>set p1. fvc_program s) \<union> (\<Union>s\<in>set p2. fvc_program s)"
+  by (cheat TODO7)
+lemma fvc_program_while: "fvc_program (while c b) = fv_expression c \<union> (\<Union>s\<in>set b. fvc_program s)"
+  by (cheat TODO7)
+lemma fvc_program_qinit: "fvc_program (qinit Q e3) = fv_expression e3"
+  by (cheat TODO7)
+lemma fvc_program_qapply: "fvc_program (qapply Q e4) = fv_expression e4"
+  by (cheat TODO7)
+lemma fvc_program_measurement: "fvc_program (measurement x R e5) = set (variable_names x) \<union> fv_expression e5"
+  by (cheat TODO7)
+
+consts fvcw_program :: "program \<Rightarrow> string set"
+lemma fvcw_program_sequence: "fvcw_program (block b) = (\<Union>s\<in>set b. fvcw_program s)"
+  by (cheat TODO7)
+lemma fvcw_program_assign: "fvcw_program (assign x e) = set (variable_names x)"
+  by (cheat TODO7)
+lemma fvcw_program_sample: "fvcw_program (sample xs e2) = set (variable_names xs)"
+  by (cheat TODO7)
+lemma fvcw_program_ifthenelse: "fvcw_program (ifthenelse c p1 p2) =
+  (\<Union>s\<in>set p1. fvcw_program s) \<union> (\<Union>s\<in>set p2. fvcw_program s)"
+  by (cheat TODO7)
+lemma fvcw_program_while: "fvcw_program (while c b) = (\<Union>s\<in>set b. fvcw_program s)"
+  by (cheat TODO7)
+lemma fvcw_program_qinit: "fvcw_program (qinit Q e3) = {}"
+  by (cheat TODO7)
+lemma fvcw_program_qapply: "fvcw_program (qapply Q e4) = {}"
+  by (cheat TODO7)
+lemma fvcw_program_measurement: "fvcw_program (measurement x R e5) = set (variable_names x)"
   by (cheat TODO7)
 
 typedecl program_state
@@ -50,6 +90,9 @@ definition probability :: "bool expression \<Rightarrow> program \<Rightarrow> p
 consts "probability_syntax" :: "bool \<Rightarrow> program \<Rightarrow> program_state \<Rightarrow> real" ("Pr[_:(_'(_'))]")
 translations "CONST probability_syntax a b c" \<rightleftharpoons> "CONST probability (Expr[a]) b c"
 hide_const probability_syntax
+
+named_theorems program_bodies
+named_theorems program_fv
 
 ML_file "programs.ML"
 
